tot_serializer, pull parser/serializer to Tot

src/lowparse/LowParse.Spec.Base.fst
@@ -23,6 +23,15 @@ let parser_kind_prop_ext
 = no_lookahead_ext f1 f2;
   injective_ext f1 f2
 
+let tot_parser_of_parser
+  #k
+  #t
+  p
+= let p' : tot_bare_parser t = Ghost.reveal (FStar.Ghost.Pull.pull p) in
+  assert (forall x . p' x == p x);
+  parser_kind_prop_ext k p p';
+  p'
+
 let is_weaker_than_correct
   (k1: parser_kind)
   (k2: parser_kind)
@@ -95,6 +104,10 @@ let serializer_correct_implies_complete
     assert (injective_postcond p (f x) s)
   in
   Classical.forall_intro (Classical.move_requires prf)
+
+let tot_serializer_of_serializer
+  s
+= FStar.Ghost.Pull.pull s
 
 let serializer_parser_unique'
   (#k1: parser_kind)
